\begin{remark}
  By dependent choice, for any sequence of finite sets $(X_n)_{n:\N}$
  we can merely find a sequence $l : \N \to \N$ such that $||X_n = Fin(l_n)||$.
  Thus we have a surjection 
  $$\left(\sum_{l:\N\to\N} \prod_{k:\N}\Fin(l_{k+1}) \to 
  \Fin(l_k)\right) \twoheadrightarrow \Stone$$
  sending a sequence 
  $\begin{tikzcd}
    Fin(l_0) & Fin(l_1) \arrow[l, "\gamma_0"'] & Fin (l_2) \arrow[l , "\gamma_1"'] & \cdots \arrow[l, "\gamma_2"']
  \end{tikzcd}$
  to it's limit. 

  Note that the limit of a sequence is inhabited if and only if $l_k$ is positive 
  for all $ k : \N$. 
  Therefore, this above surjection restricts to a surjection 
  $$\alpha : \left(\sum_{l:\N\to\N_+} \prod_{k:\N}\Fin(l_{k+1}) \to 
  \Fin(l_k)\right) \twoheadrightarrow \sum_{X:\Stone}\propTrunc{X}.$$ 
\end{remark} 


\begin{lemma}
For $S:\Stone$, any map $T:S\to \sum_{X:\Stone}\propTrunc{X}$ 
merely factors through $\alpha$ above.
\end{lemma}
\begin{proof}
  By Theorem 4.18 of \cite{condensed-foundations}, 
  the total space $\Sigma_{s : S} T(s)$ is Stone. 
  Note that as $T$ lands in inhabited Stone spaces, 
  the projection map $\pi_S : \Sigma_{s : S} T(s) \to S$ is surjective. 
  By Remark 3.4 of \cite{condensed-foundations} and dependent choice, 
  we can write $\pi_S$ as sequential limits of surjections
  $\pi_{S,n} : Fin(\alpha_n) \twoheadrightarrow Fin(\beta_n)$ for some sequences 
  $\alpha,\beta : \N \to \N$. Write $\cdot|_n$ for the map $S \to Fin(\alpha_n)$. 
  
  Now fix $s:S$.
  Note that $T(s)$ is the fiber of $\pi_S$ at $s$. 
  Furthermore, the fiber is a limit, hence commutes with sequential limits, so 
  $T(s)$ is the limit of the fibers of $\pi_{S,n}$ at $s|_n$.

  Now the fiber of a map between finite sets is finite. 
  Let $\beta : \N \to \N$ denote the size of $\pi_{S,n}^{-1}(s|_n)$. 
  The order on $Fin(\alpha_n)$ induces an explicit equivalence between 
  $\pi_{S,n}^{-1}(s|_n)$ and $Fin(\beta_n)$. 
  We now have that $T(s) $ is the limit of $Fin(\beta_n)$.
  As $T(s)$ is inhabited, we have that $\beta_n >0$ for all $n$, 
  and we get the desired result. 
\end{proof}
  







% Thus there exists sequences $t, s : \mathbb N \to \mathbb N$ with maps
% $\Pi_{n : \N} Fin(t_{n+1}) \to Fin(t_n), 
% \Pi_{n : \N} Fin(s_{n+1}) \to Fin(s_n), 
% \Pi_{n : \N} Fin(t_n) \to Fin(s_n)$ 
%  such that
%  \begin{equation}\begin{tikzcd}
%    Fin(t_0) \arrow[d, two heads] & Fin (t_1) \arrow[l] \arrow[d, two heads] & 
%    \arrow[l]\cdots & \arrow[l] \arrow[d, two heads] Fin (t_n) & \cdots \arrow[l] & 
%    \arrow[ l ] \arrow [d, two heads ]\Sigma_{s : S} T(s)\\
%    Fin(s_0) & Fin (s_1) \arrow[l] & \cdots \arrow[l] & \arrow[l] Fin (s_n) & 
%    \cdots \arrow[l] & \arrow[ l ] S\\
%  \end{tikzcd}\end{equation}  
