\subsection{First cohomology vanish for Stone spaces}

First some result on \v{C}ech sequences and cohomology. It works in plain HoTT and is certainly not new.

\begin{lemma}\label{cocyle-being-coboundary}
Assume given sets $S,S'$ with a surjection:
\[S'\to S\]
and write $T(x)$ its fiber over $X:S$.

Assume given $A:S\to \mathrm{Ab}$ with:
\[\phi:\prod_{x:S}BA(x)\]
and:
\[\alpha:\prod_{x:S}(\phi(x)=*)^{T(x)}\]
If the beginning of the \v{C}ech sequence:
\[\prod_{x:S}A(x)^{T(x)} \to \prod_{x:S}A(x)^{T(x)^2}  \to \prod_{x:S}A(x)^{T(x)^3} \]
is exact then $\phi=*$.
\end{lemma}

\begin{proof}
See \cref{cech-sequence-definition} for the definition of the maps in the sequence.

We define:
\[g : \prod_{x:S}T(x)^2\to A(x)\]
by having $g_x(y,z)$ the the element $\alpha_x(y)^{-1}\cdot\alpha_x(z)$. It is easy to check that it is a cocycle in the given sequence, so that by exactness there is $f:\prod_{x:S}T(x)\to A(x)$ such that for all $x:S$ and $y,z:T(x)$ we have that:
\[g_x(y,z)=f_x(y)\cdot f_x(z)^{-1}\]
Then we define:
\[\alpha' : \prod_{x:S}(\phi(x)=*)^{T(x)}\]
\[\alpha'_x(y) = \alpha_x(y)\cdot f_x(y)\]
so that for all $x:S$ and $y,z:T(x)$ we have that:
\[\alpha'_x(z)^{-1}\cdot\alpha'_x(y) = f_x(z)^{-1}\alpha_x(z)^{-1}\alpha_x(y)\cdot f_x(y) = \mathrm{refl}\]
so that:
\[\alpha'_x(y)=\alpha'_x(z)\]
and this means that $\alpha'$ factors through $S$, giving a proof of $\phi=*$.
\end{proof}

We prove the \v{C}ech sequence of a map to a finite type is exact:

\begin{lemma}\label{vanishing-cech-finite-types}
Assume $F$ finite type with a type $X$ and a surjective map $q:X\to F$. We write $I(x)$ the fibers of $q$ over $x:F$. 

Assume given $A:F\to \mathrm{Ab}$, then the \v{C}ech sequence:
\[\prod_{x:F}A(x)^{I(x)} \to \prod_{x:F}A(x)^{I(x)^2}  \to \prod_{x:F}A(x)^{I(x)^3} \]
is exact.
\end{lemma}

\begin{proof}
Since $F$ is finite and exactness is stable under finite products, we can assume $F=1$, then $A$ is just an abelian group and $I$ an inhabited type, say with $0:I$. Then we are considering the sequence:
\[A^I \to A^{I^2} \to A^{I^3}\]
with the maps:
\[(a_i)_{i:I} \mapsto (a_i-a_j)_{i,j:I}\]
\[(a_{i,j})_{i,j:I} \mapsto (a_{i,j}+a_{j,k}-a_{i,k})_{i,j,k:I}\]
Assume $(a_{i,j})_{i,j:I}$ such that for all $i,j,k:I$ we have that $a_{i,j}+a_{j,k}=a_{i,k}$. 

First we have that $a_{i,i}+a_{i,i}=a_{i,i}$ so that $a_{i,i}=0$. Then $a_{i,j}+a_{j,i} = a_{i,i}$ gives that $a_{i,j} = -a_{j,i}$. Now we consider $(a_{i,0})_{i:I}$, which is sends to $(a_{i,0}-a_{j,0})_{i,j:I} = (a_{i,j})_{i,j:I}$. So the sequence is indeed exact.
\end{proof}

We want to prove that the vanishing of the \v{C}ech sequence of Stone spaces with overtly discrete coefficients is stable under sequential limit. It will rely heavily on Scott continuity. We need an auxiliary definition:

\begin{definition}
Assume given $S = \lim_kS_k$ sequential limits of Stone and $A:S\to \mathrm{Ab}_\ODisc$. Then we define:
\[A_k: S_k\to \mathrm{Ab}_{\ODisc}\]
\[A_k(x) = \prod_{y:S,y|_k=x} A(y)\]
By the dual to Tychonov, we have that $A_k(x)$ is overtly discrete. 

Moreover we for all $k:\N$ and $x:S_{k+1}$ we have a map:
\[A_k(x|_k) \to A_{k+1}(x)\]
\end{definition}

The two references in the proof are to variants of Scott continuity, in the directed univalence draft.

\begin{lemma}\label{vanishing-cech-stable-sequential-limits}
Assume given $S=\lim_kS_k$ and $S'=\lim_kS'_k$ limits of Stone spaces, and a surjective map of towers:
\begin{center}
\begin{tikzcd}
S_0' \ar[d] & S_1'\ar[l]\ar[d] & S_2'\ar[d]\ar[l]& \cdots\ar[l] \\
S_0 & S_1\ar[l] & S_2 \ar[l]& \cdots\ar[l] \\
\end{tikzcd}
\end{center}

We denote the fibers of the induced map $S'\to S$ over $x:S$ by $T(x)$ and the fibers of the map $S_k'\to S_k$ over $x:S_k$ by $T_k(x)$.

Assume given $A:S\to\mathrm{Ab}_\ODisc$ such that for all $k:\N$ the \v{C}ech sequence:
\[\prod_{x:S_k}A_k(x)^{T_k(x)} \to \prod_{x:S_k}A_k(x)^{T_k(x)^2}  \to \prod_{x:S_k}A_k(x)^{T_k(x)^3} \]
is exact. Then the \v{C}ech sequence:
\[\prod_{x:S}A(x)^{T(x)} \to \prod_{x:S}A(x)^{T(x)^2}  \to \prod_{x:S}A(x)^{T(x)^3} \]
is exact.
\end{lemma}

\begin{proof}
We prove that for any $l:\N$ we have that:
\[\mathrm{colim}_k \left(\prod_{x:S_k}A_k(x)^{T_k(x)^l}\right)  = \prod_{x:S}A(x)^{T(x)^l} \]
We conclude from this and exactness being stable under sequential colimit. We omit the verification that this is compatible with maps. 

We have that:
\[\prod_{x:S_k}A_k(x)^{T_k(x)^l} = \prod_{x:S_k}\prod_{y:S,y|_k=x} A(y)^{T_k(x)^l} = \prod_{y:S} A(y)^{T_k(y|_k)^l}\]
and by \cref{scott-continuity-right} we have that:
\[\mathrm{colim}_k\left(\prod_{y:S} A(y)^{T_k(y|_k)^l}\right) = \prod_{y:S} \mathrm{colim}_k\left( A(y)^{T_k(y|_k)^l} \right)\]
but by \cref{scott-continuity} we have that:
\[\mathrm{colim}_k\left( A(y)^{T_k(y|_k)^l} \right) = A(y)^{\lim_k T_k(y|_k)^l}\]
and we can see by commutation of limits that:
\[\lim_k T_k(y|_k)^l = T(y)^l\]
\end{proof}

Now we just have to assemble the pieces.

\begin{lemma}\label{vanishing-1-cohomology-stone}
Let $S$ be Stone and $A: S\to \mathrm{Ab}_\ODisc$. Then:
\[H^1(S,A) = 0\]
\end{lemma}

\begin{proof}
Assume given:
\[\phi:\prod_{s:S}BA(x)\]
we have that:
\[\prod_{x:S}\propTrunc{\phi(x)=*}\]
so that by local choice there merely exists $S'$ Stone and a surjective map:
\[q:S'\to S\]
with fibers denoted $T(x)$ and:
\[\alpha:\prod_{x:S'}(\phi(x)=*)^{T(x)}\]
In order to conclude by applying \cref{cocyle-being-coboundary}, it is enough to prove that the \v{C}ech sequence:
\[\prod_{x:S}A(x)^{T(x)} \to \prod_{x:S}A(x)^{T(x)^2}  \to \prod_{x:S}A(x)^{T(x)^3} \]
is exact.

By \cref{TODO} we know that any surjective map between Stone spaces is a sequential limit of surjective maps between finite types. So by applying \cref{vanishing-cech-stable-sequential-limits} we see it is enough to prove the exactness of the exact sequence for maps between finite types, and this is \cref{vanishing-cech-finite-types}.
\end{proof}

\subsection{Stone spaces are acyclic}

We extend the previous section to the following: for all $S$ Stone,$A:S\to\mathrm{Ab}_\ODisc$ and $n>0$ we have that:
\[H^n(S,A) = 0\]
We (Thierry \& Hugo) follow David's proof in SAG to go from $1$ to all $n$.

\begin{lemma}\label{eilenberg-exponentials-auxiliary}
Assume for all $S$ Stone and $A:\mathrm{Ab}_\ODisc$ we have that:
\[H^k(S,A) = 0\] 
for all $0<k<n$. Then:
\begin{itemize}
\item For all $S$ Stone and $A$ overtly discrete abelian group, for all $k<n$ the map:
\[K(A^S,k) \to K(A,k)^S\]
is an equivalence.
\item For all $S$ Stone and $A$ overtly discrete abelian group, the map:
\[K(A^S,n) \to K(A,n)^S\]
is an embedding.
\end{itemize}
\end{lemma}

\begin{proof}
We proceed by induction on $n$. If $n=0$ this is clear as we always have that $K(A^S,0) = K(A,0)^S$.

Assume it holds for $n$, then:
\begin{itemize} 
\item We need to prove that the embedding:
\[K(A^S,n) \to K(A,n)^S\]
is an equivalence. If $n=0$ it is immediate and otherwise by $H^n(S,A)=0$ we know that $K(A,n)^S$ is connected, so the embedding is surjective and therefore an equivalence. 
\item We need to prove that the map:
\[K(A^S,n+1) \to K(A,n+1)^S\]
is an embedding, since the source is connected it is enough to prove that:
\[\Omega K(A^S,n+1) \to \Omega (K(A,n+1)^S)\]
is an equivalence but this is the previous bullet-point.
\end{itemize}
\end{proof}

\begin{theorem}\label{vanishing-cohomology-stone}
Let $S$ be Stone and $A:S\to\mathrm{Ab}_\ODisc$. Then for all $n>0$ we have that:
\[H^n(S,A) = 0\]
\end{theorem}

\begin{proof}
We proceed by induction on $k$. For $k=1$ it is \cref{vanishing-1-cohomology-stone}.

Assume it hold for all $0<k<n$ we want to prove it for $n$. Assume:
\[\alpha : \prod_{x:S} K(A_x,k+1)\]
By local choice we have a surjective map:
\[f:\sum_{x:S}T_x\to S\]
with $T_x$ Stone such that we merely have:
\[\prod_{x:S} T_x\to (\alpha(x) = *)\]
This means that the image of $\alpha$ under the diagonal map:
\[\prod_{x:S} K(A_x,k+1) \to \prod_{x:S} K(A_x,k+1)^{T_x}\]
merely is zero.

By \cref{eilenberg-exponentials-auxiliary} it means that the image of $\alpha$ by the map:
\[\prod_{x:S} K(A_x,n) \to \prod_{x:S} K(A_x^{T_x},n)\]
merely is $0$, which means that the map:
\[H^{n}(x:S,A_x) \to H^{n}(x:S,A_x^{T_x})\]
sends $\alpha$ to $0$. 

Then we consider the exact sequence depending on $x:S$:
\[0\to A_x\to A_x^{T_x}\to L_x\to 0\]
so we have an exact sequence: 
\[H^{n-1}(x:S,L_x)\to H^n(x:S,A_x)\to H^n(x:S,A_x^{T_x})\]
where $\alpha$ is send to $0$ in $H^n(x:S,A_x^{T_x})$. By induction we have $H^{n-1}(x:S,L_x)$ from which we conclude that $\alpha$ is equal to $0$ in $H^n(x:S,A_x)$.
\end{proof}

\begin{corollary}\label{eilenberg-exponentials}
For all $S$ Stone, $A:\mathrm{Ab}_\ODisc$ and $n$ we have that the map:
\[K(A^S,n) \to K(A,n)^S\]
is an equivalence.
\end{corollary}

\begin{proof}
From \cref{eilenberg-exponentials-auxiliary} and \cref{vanishing-cohomology-stone}.
\end{proof}


\subsection{\v{C}ech cohomology}

\begin{definition}
A \v{C}ech cover for a type $X$ consists of a surjective map:
\[f:S\to X\]
where $S$ is Stone and for all $x:X$ the fiber $S_x$ of $f$ over $x$ is Stone.
\end{definition}

Next lemma show that cohomology interact well with \v{C}ech cover. It will be used later to prove that cohomology and \v{C}ech cohomology agree.

\begin{lemma}\label{inductive-definition-cohomology}
Assume given $X$ a type with a \v{C}ech cover:
\[f:S\to X\]
as well as $A:X\to \mathrm{Ab}_\ODisc$.

For all $n\geq 1$ we have an exact sequence:
\[H^{n-1}(X,x\mapsto A_x^{S_x}) \to H^{n-1}(X,L)\to H^n(X,A)\to 0\]
natural in $A$, where $L_x = A_x^{S_x}/A_x$.
\end{lemma}

\begin{proof}
Using the long exact sequence associated to:
\[0\to A_x\to A_x^{S_x}\to L_x\to 0\]
by \cref{vanishing-cohomology-stone} it is enough to prove that for all $n$ we have:
\[H^n(x:X,A_x^{S_x}) = H^n(x:S,A_x)\]
But by \cref{eilenberg-exponentials} we have that:
\[\prod_{x:X}K(A_x^{S_x},n) = \prod_{x:S}K(A_x,n)\]
\end{proof}

\begin{definition}\label{cech-sequence-definition}
Assume given a \v{C}ech cover
\[f:S\to X\]
and $A:X\to\mathrm{Ab}_\ODisc$.

Then we define the \v{C}ech complex by:
\[\prod_{x:X}A_x^{S_x} \to \prod_{x:X}A_x^{S_x\times S_x} \to \cdots\]
with the boundary maps defined as expected, that is:
\[\delta(\alpha)(x,u_0,\cdots,u_n) = \sum_{i=0}^n (-1)^i\alpha(x,u_0,\cdots,\hat{u_i},\cdots,u_n)\]
Then the \v{C}ech cohomology:
\[\check{H}^k(x:X,A_x)\]
is defined as the $k$-th homology group of the \v{C}ech complex.
\end{definition}

\begin{lemma}
Assume given a \v{C}ech cover:
\[f:S\to X\]
If we are given a short exact sequence of overtly discrete abelian group:
\[0\to A_x\to B_x\to C_x\to 0\]
depending on $x:X$, there is a long exact sequence of \v{C}ech cohomology groups:
\[\check{H}^0(X,A) \to\check{H}^0(X,B) \to\check{H}^0(X,C) \to\check{H}^1(X,A) \to\check{H}^1(X,B) \to\check{H}^1(X,C) \to\cdots \]
Moreover this long exact sequence is natural in the short exact sequence.
\end{lemma}

\begin{proof}
We just use the fact that all elements $\sum_{x:X} T_x^{k+1}$ in the \v{C}ech complex are Stone spaces, so a short exact sequence of overtly discrete abelian group induces a short exact of \v{C}ech complexes by \cref{vanishing-cohomology-stone}.
\end{proof}

\begin{lemma}\label{inductive-definition-cech-cohomology}
Assume given a \v{C}ech cover:
\[f:S\to X\]
and $A:X\to\mathrm{Ab}_\ODisc$.

For all $n\geq 1$ we have an exact sequence:
\[\check{H}^{n-1}(X,x\mapsto A_x^{S_x}) \to \check{H}^{n-1}(X,L)\to \check{H}^n(X,A)\to 0\]
natural in $A$ where $L_x=A_x^{S_x}/A_x$.
\end{lemma}

\begin{proof}
It is enough to prove $\check{H}^n(X,x\mapsto A_x^{S_x}) = 0$ for all $n\geq 1$. Indeed assume given:
\[\alpha : \prod_{x:X} S_x^{n+1}\to S_x\to A_x\]
such that $\delta(\alpha) = 0$, i.e. for all $x:X$ and $u_0,\cdots, u_{n+1},v:S_x$ we have that:
\[\sum_{i=0}^{n+1}(-1)^i\alpha(x,u_0,\cdots,  \hat{u_i},\cdots ,u_{n+1},v) = 0\]
Then we define:
\[\beta : \prod_{x:X} S_x^{n}\to S_x\to A_x\]
\[\beta(x,u_0,\cdots,u_{n-1},v) = (-1)^n\alpha(x,u_0,\cdots,u_{n-1},v,v)\]
and then:
\[\delta(\beta)(x,u_0,\cdots,u_{n},v) = (-1)^n\sum_{i=0}^{n} (-1)^i \alpha(x,u_0,\cdots,\hat{u_i},\cdots,u_n,v,v) \]
\[= \alpha(x,u_0,\cdots,u_n,v)\]
\end{proof}

\begin{theorem}
Assume given a \v{C}ech cover:
\[f:S\to X\]
and $A:X\to\mathrm{Ab}_\ODisc$.

Then we have a natural isomorphism:
\[H^n(X,A) = \check{H}^n(X,A)\]
\end{theorem}

\begin{proof}
We proceed by induction on $n$. For $n=0$ we need to prove that maps:
\[\alpha:\prod_{s:S}A_{f(s)}\]
such that whenever $f(s)=f(t)$ we have that $\alpha(s) = \alpha(t)$ are naturally isomorphic to:
\[\prod_{x:X}A_x\]
This is immediate.

For the inductive step we use \cref{inductive-definition-cohomology} and \cref{inductive-definition-cech-cohomology}. Naturality comes from the naturality of the exact sequences.
\end{proof}


\subsection{The unit interval is acyclic}

\begin{proposition}\label{vanishing-cohomology-interval}
For all $A$ overtly discrete and all $k$ we have that:
\[H^k(\mathbb{I},A) = 0\]
\end{proposition}

\begin{proof}
TODO
\end{proof}
